theories/case_studies/cmdc/cmdc_concrete.v
@@ -1,0 +1,332 @@
+From iris.program_logic Require Import adequacy.
+From griotte Require Import
+  machine_instructions machine_parameters machine_parameters_instance
+  registers griotte_lang machine_run switcher assert compartment_layout
+  cmdc cmdc_adequacy disjoint_regions_tactics.
+
+Existing Instance machine_parameters_instance.
+
+Local Transparent MemNum ONum.
+
+Local Notation "'A' z" :=
+  (@finz.FinZ MemNum z%Z eq_refl eq_refl) (at level 10).
+Local Notation "'OT' z" :=
+  (@finz.FinZ ONum z%Z eq_refl eq_refl) (at level 10).
+
+Definition cmdc_main_pcc_begin : Addr := A 9.
+Definition cmdc_main_code_start : Addr := A 13.
+Definition cmdc_main_pcc_end : Addr := A 98.
+Definition cmdc_B_pcc_begin : Addr := A 98.
+Definition cmdc_B_code_start : Addr := A 99.
+Definition cmdc_B_pcc_end : Addr := A 102.
+Definition cmdc_C_pcc_begin : Addr := A 102.
+Definition cmdc_C_code_start : Addr := A 103.
+Definition cmdc_C_pcc_end : Addr := A 105.
+Definition cmdc_main_data_begin : Addr := A 105.
+Definition cmdc_main_data_end : Addr := A 107.
+Definition cmdc_B_data_begin : Addr := A 107.
+Definition cmdc_B_data_end : Addr := A 108.
+Definition cmdc_C_data_begin : Addr := A 108.
+Definition cmdc_C_data_end : Addr := A 109.
+Definition cmdc_main_exports_pcc : Addr := A 109.
+Definition cmdc_main_exports_cgp : Addr := A 110.
+Definition cmdc_main_exports_entries_begin : Addr := A 111.
+Definition cmdc_main_exports_entries_end : Addr := A 111.
+Definition cmdc_B_exports_pcc : Addr := A 111.
+Definition cmdc_B_exports_cgp : Addr := A 112.
+Definition cmdc_B_exports_entries_begin : Addr := A 113.
+Definition cmdc_B_exports_entries_end : Addr := A 114.
+Definition cmdc_C_exports_pcc : Addr := A 114.
+Definition cmdc_C_exports_cgp : Addr := A 115.
+Definition cmdc_C_exports_entries_begin : Addr := A 116.
+Definition cmdc_C_exports_entries_end : Addr := A 117.
+Definition cmdc_assert_begin : Addr := A 117.
+Definition cmdc_assert_cap : Addr := A 129.
+Definition cmdc_assert_end : Addr := A 130.
+Definition cmdc_assert_flag : Addr := A 130.
+Definition cmdc_switcher_begin : Addr := A 131.
+Definition cmdc_switcher_call : Addr := A 132.
+Definition cmdc_switcher_return : Addr := A 220.
+Definition cmdc_switcher_end : Addr := A 282.
+Definition cmdc_switcher_sealing_type : OType := OT 9.
+Definition cmdc_trusted_stack_begin : Addr := A 4096.
+Definition cmdc_trusted_stack_end : Addr := A 4196.
+Definition cmdc_stack_begin : Addr := A 1024.
+Definition cmdc_stack_end : Addr := A 1124.
+
+Ltac unfold_cmdc_addresses :=
+  unfold cmdc_main_pcc_begin, cmdc_main_code_start, cmdc_main_pcc_end,
+    cmdc_B_pcc_begin, cmdc_B_code_start, cmdc_B_pcc_end,
+    cmdc_C_pcc_begin, cmdc_C_code_start, cmdc_C_pcc_end,
+    cmdc_main_data_begin, cmdc_main_data_end, cmdc_B_data_begin,
+    cmdc_B_data_end, cmdc_C_data_begin, cmdc_C_data_end,
+    cmdc_main_exports_pcc, cmdc_main_exports_cgp,
+    cmdc_main_exports_entries_begin, cmdc_main_exports_entries_end,
+    cmdc_B_exports_pcc, cmdc_B_exports_cgp, cmdc_B_exports_entries_begin,
+    cmdc_B_exports_entries_end, cmdc_C_exports_pcc, cmdc_C_exports_cgp,
+    cmdc_C_exports_entries_begin, cmdc_C_exports_entries_end,
+    cmdc_assert_begin, cmdc_assert_cap, cmdc_assert_end, cmdc_assert_flag,
+    cmdc_switcher_begin, cmdc_switcher_call, cmdc_switcher_return,
+    cmdc_switcher_end, cmdc_switcher_sealing_type,
+    cmdc_trusted_stack_begin, cmdc_trusted_stack_end,
+    cmdc_stack_begin, cmdc_stack_end.
+
+Ltac unfold_cmdc_addresses_in H :=
+  unfold cmdc_main_pcc_begin, cmdc_main_code_start, cmdc_main_pcc_end,
+    cmdc_B_pcc_begin, cmdc_B_code_start, cmdc_B_pcc_end,
+    cmdc_C_pcc_begin, cmdc_C_code_start, cmdc_C_pcc_end,
+    cmdc_main_data_begin, cmdc_main_data_end, cmdc_B_data_begin,
+    cmdc_B_data_end, cmdc_C_data_begin, cmdc_C_data_end,
+    cmdc_main_exports_pcc, cmdc_main_exports_cgp,
+    cmdc_main_exports_entries_begin, cmdc_main_exports_entries_end,
+    cmdc_B_exports_pcc, cmdc_B_exports_cgp, cmdc_B_exports_entries_begin,
+    cmdc_B_exports_entries_end, cmdc_C_exports_pcc, cmdc_C_exports_cgp,
+    cmdc_C_exports_entries_begin, cmdc_C_exports_entries_end,
+    cmdc_assert_begin, cmdc_assert_cap, cmdc_assert_end, cmdc_assert_flag,
+    cmdc_switcher_begin, cmdc_switcher_call, cmdc_switcher_return,
+    cmdc_switcher_end, cmdc_switcher_sealing_type,
+    cmdc_trusted_stack_begin, cmdc_trusted_stack_end,
+    cmdc_stack_begin, cmdc_stack_end in H.
+
+(** The concrete adversary consists of two unknown compartments. Compartment
+    [B] writes [7] through the capability it receives and also saves that
+    capability on its stack; compartment [C] writes [9] through its received
+    capability. Together they exercise the main program's cross-compartment
+    capability discipline. *)
+Definition cmdc_B_code : list Word :=
+  encodeInstrsW [Store ca0 7%Z; Store csp ca0; Jalr cnull cra].
+Definition cmdc_C_code : list Word :=
+  encodeInstrsW [Store ca0 9%Z; Jalr cnull cra].
+Definition cmdc_B_data : list Word := [WInt 0].
+Definition cmdc_C_data : list Word := [WInt 0].
+Definition cmdc_B_imports : list Word :=
+  [WSentry XSRW_ Local cmdc_switcher_begin cmdc_switcher_end cmdc_switcher_call].
+Definition cmdc_C_imports : list Word :=
+  [WSentry XSRW_ Local cmdc_switcher_begin cmdc_switcher_end cmdc_switcher_call].
+Definition cmdc_B_exports : list Word := [WInt (encode_entry_point 1 1)].
+Definition cmdc_C_exports : list Word := [WInt (encode_entry_point 1 1)].
+
+Program Definition cmdc_concrete_cmptSwitcher : cmptSwitcher.
+Proof.
+  refine (@mkCmptSwitcher machine_parameters_instance
+    cmdc_switcher_begin cmdc_switcher_end cmdc_switcher_call
+    cmdc_switcher_return cmdc_switcher_sealing_type
+    cmdc_trusted_stack_begin cmdc_trusted_stack_end _ _ _ _
+    (replicate 100 (WInt 0)) _ eq_refl cmdc_stack_begin cmdc_stack_end
+    (replicate 100 (WInt 0)) _ _).
+  - vm_compute; solve_addr.
+  - vm_compute; solve_addr.
+  - vm_compute; solve_addr.
+  - vm_compute; solve_addr.
+  - vm_compute; solve_addr.
+  - vm_compute; solve_addr.
+  - unfold_cmdc_addresses.
+    repeat split; unfold disjoint, set_disjoint_instance;
+      intros x Hx Hx'; rewrite !elem_of_finz_seq_between in Hx, Hx';
+      solve_addr.
+Defined.
+
+Program Definition cmdc_concrete_cmptAssert : cmptAssert.
+Proof.
+  refine (@mkCmptAssert machine_parameters_instance cmdc_assert_begin
+    cmdc_assert_end cmdc_assert_cap cmdc_assert_flag _ _ _ _).
+  - vm_compute; solve_addr.
+  - vm_compute; solve_addr.
+  - vm_compute; solve_addr.
+  - unfold_cmdc_addresses.
+    unfold disjoint, set_disjoint_instance.
+    intros x Hx Hx'.
+    rewrite !elem_of_finz_seq_between in Hx, Hx'.
+    solve_addr.
+Defined.
+
+Local Instance cmdc_concrete_switcherLayout : switcherLayout.
+Proof.
+  exact (cmptSwitcher_switcherLayout cmdc_concrete_cmptSwitcher).
+Defined.
+
+Local Instance cmdc_concrete_assertLayout : assertLayout.
+Proof.
+  exact (cmptAssert_assertLayout cmdc_concrete_cmptAssert).
+Defined.
+
+Definition cmdc_B_f : Sealable :=
+  SCap RO Global cmdc_B_exports_pcc cmdc_B_exports_entries_end
+    cmdc_B_exports_entries_begin.
+Definition cmdc_C_g : Sealable :=
+  SCap RO Global cmdc_C_exports_pcc cmdc_C_exports_entries_end
+    cmdc_C_exports_entries_begin.
+Definition cmdc_main_imports_concrete : list Word :=
+  cmdc_main_imports cmdc_B_f cmdc_C_g.
+
+Program Definition cmdc_concrete_main_cmpt : cmpt.
+Proof.
+  refine (@mkCmpt cmdc_main_pcc_begin cmdc_main_code_start cmdc_main_pcc_end
+    cmdc_main_data_begin cmdc_main_data_end cmdc_main_exports_pcc
+    cmdc_main_exports_cgp cmdc_main_exports_entries_begin
+    cmdc_main_exports_entries_end cmdc_main_imports_concrete cmdc_main_code
+    cmdc_main_data [] _ _ _ _ _ _ _).
+  - vm_compute; solve_addr.
+  - vm_compute; solve_addr.
+  - vm_compute; solve_addr.
+  - vm_compute; solve_addr.
+  - vm_compute; solve_addr.
+  - vm_compute; solve_addr.
+  - unfold_cmdc_addresses; disj_regions.
+Defined.
+
+Program Definition cmdc_concrete_B_cmpt : cmpt.
+Proof.
+  refine (@mkCmpt cmdc_B_pcc_begin cmdc_B_code_start cmdc_B_pcc_end
+    cmdc_B_data_begin cmdc_B_data_end cmdc_B_exports_pcc cmdc_B_exports_cgp
+    cmdc_B_exports_entries_begin cmdc_B_exports_entries_end cmdc_B_imports
+    cmdc_B_code cmdc_B_data cmdc_B_exports _ _ _ _ _ _ _).
+  - vm_compute; solve_addr.
+  - vm_compute; solve_addr.
+  - vm_compute; solve_addr.
+  - vm_compute; solve_addr.
+  - vm_compute; solve_addr.
+  - vm_compute; solve_addr.
+  - unfold_cmdc_addresses; disj_regions.
+Defined.
+
+Program Definition cmdc_concrete_C_cmpt : cmpt.
+Proof.
+  refine (@mkCmpt cmdc_C_pcc_begin cmdc_C_code_start cmdc_C_pcc_end
+    cmdc_C_data_begin cmdc_C_data_end cmdc_C_exports_pcc cmdc_C_exports_cgp
+    cmdc_C_exports_entries_begin cmdc_C_exports_entries_end cmdc_C_imports
+    cmdc_C_code cmdc_C_data cmdc_C_exports _ _ _ _ _ _ _).
+  - vm_compute; solve_addr.
+  - vm_compute; solve_addr.
+  - vm_compute; solve_addr.
+  - vm_compute; solve_addr.
+  - vm_compute; solve_addr.
+  - vm_compute; solve_addr.
+  - unfold_cmdc_addresses; disj_regions.
+Defined.
+
+Ltac solve_cmdc_concrete_disjoint :=
+  unfold disjoint_cmpt, switcher_cmpt_disjoint, assert_cmpt_disjoint,
+       assert_switcher_disjoint, cmpt_region, cmpt_pcc_region, cmpt_cgp_region,
+       cmpt_exp_tbl_region, cmpt_switcher_region, cmpt_switcher_code_region,
+       cmpt_switcher_trusted_stack_region, cmpt_switcher_stack_region,
+       cmpt_assert_region, cmpt_assert_code_region, cmpt_assert_cap_region,
+       cmpt_assert_flag_region, cmdc_concrete_cmptSwitcher,
+       cmdc_concrete_cmptAssert, cmdc_concrete_main_cmpt,
+       cmdc_concrete_B_cmpt, cmdc_concrete_C_cmpt;
+  cbn [cmpt_b_pcc cmpt_e_pcc cmpt_b_cgp cmpt_e_cgp
+       cmpt_exp_tbl_pcc cmpt_exp_tbl_entries_end b_switcher e_switcher
+       b_trusted_stack e_trusted_stack b_stack e_stack b_assert cap_assert
+       e_assert flag_assert];
+  intros x Hx Hx';
+  repeat (rewrite elem_of_app in Hx || rewrite elem_of_app in Hx');
+  repeat (rewrite elem_of_finz_seq_between in Hx ||
+          rewrite elem_of_finz_seq_between in Hx');
+  unfold_cmdc_addresses_in Hx;
+  unfold_cmdc_addresses_in Hx';
+  naive_solver (solve_addr).
+
+Global Instance cmdc_concrete_layout : memory_layout.
+Proof.
+  refine (@Build_memory_layout machine_parameters_instance
+    cmdc_concrete_cmptSwitcher cmdc_concrete_cmptAssert
+    cmdc_concrete_main_cmpt cmdc_concrete_B_cmpt 1
+    cmdc_concrete_C_cmpt 1 _ _ _ _).
+  - repeat split; solve_cmdc_concrete_disjoint.
+  - repeat split; solve_cmdc_concrete_disjoint.
+  - repeat split; solve_cmdc_concrete_disjoint.
+  - solve_cmdc_concrete_disjoint.
+Defined.
+
+Definition cmdc_initial_registers : Reg :=
+  <[PC := WCap RX Global cmdc_main_pcc_begin cmdc_main_pcc_end
+      cmdc_main_code_start]>
+  (<[cgp := WCap RW Global cmdc_main_data_begin cmdc_main_data_end
+      cmdc_main_data_begin]>
+  (<[csp := WCap RWL Local cmdc_stack_begin cmdc_stack_end cmdc_stack_begin]>
+    (gset_to_gmap (WInt 0) all_registers_s))).
+
+Definition cmdc_initial_sregisters : SReg :=
+  <[MTDC := WCap RWL Local cmdc_trusted_stack_begin cmdc_trusted_stack_end
+      cmdc_trusted_stack_begin]> ∅.
+
+Definition cmdc_initial_memory : Mem := mk_initial_memory.
+
+Lemma cmdc_initial_registers_correct :
+  is_initial_registers cmdc_initial_registers.
+Proof.
+  rewrite /is_initial_registers /cmdc_initial_registers.
+  cbn [cmdc_concrete_layout cmdc_concrete_main_cmpt].
+  split; [|split; [|split]].
+  - vm_compute; reflexivity.
+  - vm_compute; reflexivity.
+  - vm_compute; reflexivity.
+  - intros r Hr; rewrite !lookup_insert_ne; try set_solver.
+    apply lookup_gset_to_gmap_Some; split.
+    + apply all_registers_s_correct.
+    + done.
+Qed.
+
+Lemma cmdc_initial_sregisters_correct :
+  is_initial_sregisters cmdc_initial_sregisters.
+Proof.
+  rewrite /is_initial_sregisters /cmdc_initial_sregisters.
+  cbn [cmdc_concrete_layout cmdc_concrete_cmptSwitcher].
+  simplify_map_eq; vm_compute; reflexivity.
+Qed.
+
+Lemma cmdc_initial_memory_correct :
+  is_initial_memory cmdc_initial_memory.
+Proof.
+  rewrite /is_initial_memory /cmdc_initial_memory.
+  repeat split; try reflexivity.
+  - rewrite /cmdc_B_code /encodeInstrsW; repeat constructor; done.
+  - rewrite /cmdc_B_data; repeat constructor; done.
+  - rewrite /cmdc_C_code /encodeInstrsW; repeat constructor; done.
+  - rewrite /cmdc_C_data; repeat constructor; done.
+Qed.
+
+Theorem cmdc_concrete_adequacy reg' sreg' mem' es :
+  rtc erased_step
+    ([Seq (Instr Executable)],
+      (cmdc_initial_registers, cmdc_initial_sregisters, cmdc_initial_memory))
+    (es, (reg', sreg', mem')) ->
+  mem' !! cmdc_assert_flag = Some (WInt 0%Z).
+Proof.
+  intro Hrun.
+  pose proof
+    (@cmdc_adequacy machine_parameters_instance cmdc_concrete_layout
+      cmdc_initial_registers reg' cmdc_initial_sregisters sreg'
+      cmdc_initial_memory mem' es cmdc_initial_registers_correct
+      cmdc_initial_sregisters_correct cmdc_initial_memory_correct Hrun)
+    as Hadequacy.
+  cbn [cmdc_concrete_layout cmdc_concrete_cmptAssert] in Hadequacy.
+  exact Hadequacy.
+Qed.
+
+(** Combining the computed execution with [cmdc_concrete_adequacy] shows that
+    there is a final machine state such that the exact initial configuration:
+    - executes to [Halted], rather than failing or exhausting the chosen fuel;
+    - finishes with the assertion flag still set to zero.
+    Thus this particular adversarial execution terminates normally without
+    violating the case study's assertion. *)
+Theorem cmdc_runs_and_gracefully_halts :
+  ∃ reg' sreg' mem',
+    rtc erased_step
+      ([Seq (Instr Executable)],
+        (cmdc_initial_registers, cmdc_initial_sregisters,
+         cmdc_initial_memory))
+      ([Instr Halted], (reg', sreg', mem'))
+    ∧ mem' !! cmdc_assert_flag = Some (WInt 0%Z).
+Proof.
+  edestruct (
+    machine_run_correct 10000 Executable
+      (cmdc_initial_registers, cmdc_initial_sregisters,
+       cmdc_initial_memory)
+      Halted
+  ) as [[[reg' sreg'] mem'] Hsteps].
+  { vm_compute; reflexivity. }
+  exists reg', sreg', mem'. split.
+  - exact Hsteps.
+  - eapply cmdc_concrete_adequacy. exact Hsteps.
+Qed.
