theories/case_studies/dle/deep_locality_concrete.v
@@ -1,0 +1,318 @@
+From iris.program_logic Require Import adequacy.
+From griotte Require Import
+  machine_instructions machine_parameters machine_parameters_instance
+  registers griotte_lang machine_run switcher assert compartment_layout
+  deep_locality deep_locality_adequacy
+  disjoint_regions_tactics.
+
+Existing Instance machine_parameters_instance.
+
+Local Transparent MemNum ONum.
+
+Local Notation "'A' z" :=
+  (@finz.FinZ MemNum z%Z eq_refl eq_refl) (at level 10).
+Local Notation "'OT' z" :=
+  (@finz.FinZ ONum z%Z eq_refl eq_refl) (at level 10).
+
+Definition dle_main_pcc_begin : Addr := A 9.
+Definition dle_main_code_start : Addr := A 12.
+Definition dle_main_pcc_end : Addr := A 67.
+Definition dle_main_data_begin : Addr := A 74.
+Definition dle_main_data_end : Addr := A 76.
+Definition dle_main_exports_pcc : Addr := A 77.
+Definition dle_main_exports_cgp : Addr := A 78.
+Definition dle_main_exports_entries_begin : Addr := A 79.
+Definition dle_main_exports_entries_end : Addr := A 79.
+
+Definition dle_C_pcc_begin : Addr := A 67.
+Definition dle_C_code_start : Addr := A 68.
+Definition dle_C_pcc_end : Addr := A 74.
+Definition dle_C_data_begin : Addr := A 76.
+Definition dle_C_data_end : Addr := A 77.
+Definition dle_C_exports_pcc : Addr := A 79.
+Definition dle_C_exports_cgp : Addr := A 80.
+Definition dle_C_exports_entries_begin : Addr := A 81.
+Definition dle_C_exports_entries_end : Addr := A 82.
+
+Definition dle_assert_begin : Addr := A 82.
+Definition dle_assert_cap : Addr := A 94.
+Definition dle_assert_end : Addr := A 95.
+Definition dle_assert_flag : Addr := A 95.
+
+Definition dle_switcher_begin : Addr := A 96.
+Definition dle_switcher_call : Addr := A 97.
+Definition dle_switcher_return : Addr := A 185.
+Definition dle_switcher_end : Addr := A 247.
+Definition dle_switcher_sealing_type : OType := OT 9.
+
+Definition dle_trusted_stack_begin : Addr := A 4096.
+Definition dle_trusted_stack_end : Addr := A 4196.
+Definition dle_stack_begin : Addr := A 1024.
+Definition dle_stack_end : Addr := A 1124.
+
+Ltac unfold_dle_addresses :=
+  unfold dle_main_pcc_begin, dle_main_code_start, dle_main_pcc_end,
+    dle_main_data_begin, dle_main_data_end, dle_main_exports_pcc,
+    dle_main_exports_cgp, dle_main_exports_entries_begin,
+    dle_main_exports_entries_end, dle_C_pcc_begin, dle_C_code_start,
+    dle_C_pcc_end, dle_C_data_begin, dle_C_data_end, dle_C_exports_pcc,
+    dle_C_exports_cgp, dle_C_exports_entries_begin,
+    dle_C_exports_entries_end, dle_assert_begin, dle_assert_cap,
+    dle_assert_end, dle_assert_flag, dle_switcher_begin, dle_switcher_call,
+    dle_switcher_return, dle_switcher_end, dle_switcher_sealing_type,
+    dle_trusted_stack_begin, dle_trusted_stack_end, dle_stack_begin,
+    dle_stack_end.
+
+Ltac unfold_dle_addresses_in H :=
+  unfold dle_main_pcc_begin, dle_main_code_start, dle_main_pcc_end,
+    dle_main_data_begin, dle_main_data_end, dle_main_exports_pcc,
+    dle_main_exports_cgp, dle_main_exports_entries_begin,
+    dle_main_exports_entries_end, dle_C_pcc_begin, dle_C_code_start,
+    dle_C_pcc_end, dle_C_data_begin, dle_C_data_end, dle_C_exports_pcc,
+    dle_C_exports_cgp, dle_C_exports_entries_begin,
+    dle_C_exports_entries_end, dle_assert_begin, dle_assert_cap,
+    dle_assert_end, dle_assert_flag, dle_switcher_begin, dle_switcher_call,
+    dle_switcher_return, dle_switcher_end, dle_switcher_sealing_type,
+    dle_trusted_stack_begin, dle_trusted_stack_end, dle_stack_begin,
+    dle_stack_end in H.
+
+Definition dle_C_nested_read : instr.
+Proof.
+  constructor 5.
+  - exact ct0.
+  - exact ca0.
+Defined.
+
+(** The concrete adversary examines the argument passed in [ca0]. If it is a
+    capability, the adversary follows it to the nested capability and attempts
+    to overwrite the nested cell with [7]; otherwise it simply returns. This
+    instantiates the unknown compartment with a direct attack on deep locality. *)
+Definition dle_C_code : list Word :=
+  encodeInstrsW [
+    GetWType ct0 ca0;
+    Sub ct0 ct0 (encodeWordType wt_cap);
+    Jnz 3%Z ct0;
+    dle_C_nested_read;
+    Store ct0 7%Z;
+    Jalr cnull cra
+  ].
+
+Definition dle_C_data : list Word := [WInt 0].
+
+Definition dle_C_imports : list Word :=
+  [WSentry XSRW_ Local dle_switcher_begin dle_switcher_end dle_switcher_call].
+
+Definition dle_C_exports : list Word :=
+  [WInt (encode_entry_point 1 1)].
+
+Program Definition dle_concrete_cmptSwitcher : cmptSwitcher.
+Proof.
+  refine (@mkCmptSwitcher machine_parameters_instance
+    dle_switcher_begin dle_switcher_end
+    dle_switcher_call dle_switcher_return dle_switcher_sealing_type
+    dle_trusted_stack_begin dle_trusted_stack_end
+    _ _ _ _
+    (replicate 100 (WInt 0)) _ eq_refl
+    dle_stack_begin dle_stack_end (replicate 100 (WInt 0)) _ _).
+  - vm_compute; solve_addr.
+  - vm_compute; solve_addr.
+  - vm_compute; solve_addr.
+  - vm_compute; solve_addr.
+  - vm_compute; solve_addr.
+  - vm_compute; solve_addr.
+  - unfold_dle_addresses.
+    repeat split; unfold disjoint, set_disjoint_instance;
+      intros x Hx Hx'; rewrite !elem_of_finz_seq_between in Hx, Hx';
+      solve_addr.
+Defined.
+
+Program Definition dle_concrete_cmptAssert : cmptAssert.
+Proof.
+  refine (@mkCmptAssert machine_parameters_instance
+    dle_assert_begin dle_assert_end dle_assert_cap dle_assert_flag _ _ _ _).
+  - vm_compute; solve_addr.
+  - vm_compute; solve_addr.
+  - vm_compute; solve_addr.
+  - unfold_dle_addresses.
+    unfold disjoint, set_disjoint_instance.
+    intros x Hx Hx'.
+    rewrite !elem_of_finz_seq_between in Hx, Hx'.
+    solve_addr.
+Defined.
+
+Local Instance dle_concrete_switcherLayout : switcherLayout.
+Proof.
+  exact (cmptSwitcher_switcherLayout dle_concrete_cmptSwitcher).
+Defined.
+
+Local Instance dle_concrete_assertLayout : assertLayout.
+Proof.
+  exact (cmptAssert_assertLayout dle_concrete_cmptAssert).
+Defined.
+
+Definition dle_C_f : Sealable :=
+  SCap RO Global dle_C_exports_pcc dle_C_exports_entries_end
+    dle_C_exports_entries_begin.
+
+Definition dle_main_imports_concrete : list Word :=
+  dle_main_imports dle_C_f.
+
+Program Definition dle_concrete_main_cmpt : cmpt.
+Proof.
+  refine (@mkCmpt
+    dle_main_pcc_begin dle_main_code_start dle_main_pcc_end
+    dle_main_data_begin dle_main_data_end
+    dle_main_exports_pcc dle_main_exports_cgp
+    dle_main_exports_entries_begin dle_main_exports_entries_end
+    dle_main_imports_concrete dle_main_code dle_main_data []
+    _ _ _ _ _ _ _).
+  - vm_compute; solve_addr.
+  - vm_compute; solve_addr.
+  - vm_compute; solve_addr.
+  - vm_compute; solve_addr.
+  - vm_compute; solve_addr.
+  - vm_compute; solve_addr.
+  - unfold_dle_addresses; disj_regions.
+Defined.
+
+Program Definition dle_concrete_C_cmpt : cmpt.
+Proof.
+  refine (@mkCmpt
+    dle_C_pcc_begin dle_C_code_start dle_C_pcc_end
+    dle_C_data_begin dle_C_data_end
+    dle_C_exports_pcc dle_C_exports_cgp
+    dle_C_exports_entries_begin dle_C_exports_entries_end
+    dle_C_imports dle_C_code dle_C_data dle_C_exports
+    _ _ _ _ _ _ _).
+  - vm_compute; solve_addr.
+  - vm_compute; solve_addr.
+  - vm_compute; solve_addr.
+  - vm_compute; solve_addr.
+  - vm_compute; solve_addr.
+  - vm_compute; solve_addr.
+  - unfold_dle_addresses; disj_regions.
+Defined.
+
+Ltac solve_dle_concrete_disjoint :=
+  unfold disjoint_cmpt, switcher_cmpt_disjoint, assert_cmpt_disjoint,
+       assert_switcher_disjoint, cmpt_region, cmpt_pcc_region, cmpt_cgp_region,
+       cmpt_exp_tbl_region, cmpt_switcher_region, cmpt_switcher_code_region,
+       cmpt_switcher_trusted_stack_region, cmpt_switcher_stack_region,
+       cmpt_assert_region, cmpt_assert_code_region, cmpt_assert_cap_region,
+       cmpt_assert_flag_region, dle_concrete_cmptSwitcher,
+       dle_concrete_cmptAssert, dle_concrete_main_cmpt, dle_concrete_C_cmpt;
+  cbn [cmpt_b_pcc cmpt_e_pcc cmpt_b_cgp cmpt_e_cgp
+       cmpt_exp_tbl_pcc cmpt_exp_tbl_entries_end
+       b_switcher e_switcher b_trusted_stack e_trusted_stack
+       b_stack e_stack b_assert cap_assert e_assert flag_assert];
+  intros x Hx Hx';
+  repeat (rewrite elem_of_app in Hx || rewrite elem_of_app in Hx');
+  repeat (rewrite elem_of_finz_seq_between in Hx ||
+          rewrite elem_of_finz_seq_between in Hx');
+  unfold_dle_addresses_in Hx;
+  unfold_dle_addresses_in Hx';
+  naive_solver (solve_addr).
+
+Global Instance dle_concrete_layout : memory_layout.
+Proof.
+  refine (@Build_memory_layout machine_parameters_instance
+    dle_concrete_cmptSwitcher dle_concrete_cmptAssert
+    dle_concrete_main_cmpt dle_concrete_C_cmpt _ _ _ _).
+  - solve_dle_concrete_disjoint.
+  - split; solve_dle_concrete_disjoint.
+  - split; solve_dle_concrete_disjoint.
+  - solve_dle_concrete_disjoint.
+Defined.
+
+Definition dle_initial_registers : Reg :=
+  <[PC := WCap RX Global dle_main_pcc_begin dle_main_pcc_end dle_main_code_start]>
+  (<[cgp := WCap RW Global dle_main_data_begin dle_main_data_end
+      dle_main_data_begin]>
+  (<[csp := WCap RWL Local dle_stack_begin dle_stack_end dle_stack_begin]>
+    (gset_to_gmap (WInt 0) all_registers_s))).
+
+Definition dle_initial_sregisters : SReg :=
+  <[MTDC := WCap RWL Local dle_trusted_stack_begin dle_trusted_stack_end
+      dle_trusted_stack_begin]> ∅.
+
+Definition dle_initial_memory : Mem := mk_initial_memory.
+
+Lemma dle_initial_registers_correct :
+  is_initial_registers dle_initial_registers.
+Proof.
+  rewrite /is_initial_registers /dle_initial_registers.
+  cbn [dle_concrete_layout dle_concrete_main_cmpt].
+  split; [|split; [|split]].
+  - vm_compute; reflexivity.
+  - vm_compute; reflexivity.
+  - vm_compute; reflexivity.
+  - intros r Hr; rewrite !lookup_insert_ne; try set_solver.
+    apply lookup_gset_to_gmap_Some; split.
+    + apply all_registers_s_correct.
+    + done.
+Qed.
+
+Lemma dle_initial_sregisters_correct :
+  is_initial_sregisters dle_initial_sregisters.
+Proof.
+  rewrite /is_initial_sregisters /dle_initial_sregisters.
+  cbn [dle_concrete_layout dle_concrete_cmptSwitcher].
+  simplify_map_eq; vm_compute; reflexivity.
+Qed.
+
+Lemma dle_initial_memory_correct :
+  is_initial_memory dle_initial_memory.
+Proof.
+  rewrite /is_initial_memory /dle_initial_memory.
+  repeat split; try reflexivity.
+  - rewrite /dle_C_code /encodeInstrsW;
+      repeat constructor; done.
+  - rewrite /dle_C_data; repeat constructor; done.
+  - apply Forall_replicate; done.
+Qed.
+
+Theorem dle_concrete_adequacy reg' sreg' mem' es :
+  rtc erased_step
+    ([Seq (Instr Executable)],
+      (dle_initial_registers, dle_initial_sregisters, dle_initial_memory))
+    (es, (reg', sreg', mem')) ->
+  mem' !! dle_assert_flag = Some (WInt 0%Z).
+Proof.
+  intro Hrun.
+  pose proof
+    (@dle_adequacy machine_parameters_instance dle_concrete_layout
+      dle_initial_registers reg'
+      dle_initial_sregisters sreg'
+      dle_initial_memory mem' es
+      dle_initial_registers_correct
+      dle_initial_sregisters_correct
+      dle_initial_memory_correct Hrun) as Hadequacy.
+  cbn [dle_concrete_layout dle_concrete_cmptAssert] in Hadequacy.
+  exact Hadequacy.
+Qed.
+
+(** Fuel 3000 is insufficient for this concrete run; 5000 reaches [Halted]. *)
+(** Combining the computed execution with [dle_concrete_adequacy] shows that
+    there is a final machine state such that the exact initial configuration:
+    - executes to [Halted], rather than failing or exhausting the chosen fuel;
+    - finishes with the assertion flag still set to zero.
+    Thus this particular adversarial execution terminates normally without
+    violating the case study's assertion. *)
+Theorem dle_runs_and_gracefully_halts :
+  ∃ reg' sreg' mem',
+    rtc erased_step
+      ([Seq (Instr Executable)],
+        (dle_initial_registers, dle_initial_sregisters, dle_initial_memory))
+      ([Instr Halted], (reg', sreg', mem'))
+    ∧ mem' !! dle_assert_flag = Some (WInt 0%Z).
+Proof.
+  pose proof
+    (machine_run_correct 5000 Executable
+      (dle_initial_registers, dle_initial_sregisters, dle_initial_memory)
+      Halted) as Hrun.
+  specialize (Hrun ltac:(vm_compute; reflexivity)).
+  destruct Hrun as [[[reg' sreg'] mem'] Hrun].
+  exists reg', sreg', mem'. split.
+  - exact Hrun.
+  - eapply dle_concrete_adequacy; exact Hrun.
+Qed.
