theories/case_studies/lse_downward/lse_concrete.v
@@ -1,0 +1,320 @@
+From iris.program_logic Require Import adequacy.
+From griotte Require Import
+  machine_instructions machine_parameters machine_parameters_instance
+  registers griotte_lang machine_run switcher assert compartment_layout
+  lse lse_adequacy disjoint_regions_tactics.
+
+Existing Instance machine_parameters_instance.
+Local Transparent MemNum ONum.
+
+Local Notation "'A' z" :=
+  (@finz.FinZ MemNum z%Z eq_refl eq_refl) (at level 10).
+Local Notation "'OT' z" :=
+  (@finz.FinZ ONum z%Z eq_refl eq_refl) (at level 10).
+
+Definition lse_main_pcc_begin : Addr := A 9.
+Definition lse_main_code_start : Addr := A 12.
+Definition lse_main_pcc_end : Addr := A 56.
+Definition lse_C_pcc_begin : Addr := A 56.
+Definition lse_C_code_start : Addr := A 58.
+Definition lse_C_pcc_end : Addr := A 99.
+Definition lse_main_data_begin : Addr := A 99.
+Definition lse_main_data_end : Addr := A 100.
+Definition lse_C_data_begin : Addr := A 100.
+Definition lse_C_data_end : Addr := A 101.
+Definition lse_main_exports_pcc : Addr := A 101.
+Definition lse_main_exports_cgp : Addr := A 102.
+Definition lse_main_exports_entries_begin : Addr := A 103.
+Definition lse_main_exports_entries_end : Addr := A 104.
+Definition lse_C_exports_pcc : Addr := A 104.
+Definition lse_C_exports_cgp : Addr := A 105.
+Definition lse_C_exports_entries_begin : Addr := A 106.
+Definition lse_C_exports_entries_end : Addr := A 107.
+Definition lse_assert_begin : Addr := A 107.
+Definition lse_assert_cap : Addr := A 119.
+Definition lse_assert_end : Addr := A 120.
+Definition lse_assert_flag : Addr := A 120.
+Definition lse_switcher_begin : Addr := A 121.
+Definition lse_switcher_call : Addr := A 122.
+Definition lse_switcher_return : Addr := A 210.
+Definition lse_switcher_end : Addr := A 272.
+Definition lse_switcher_sealing_type : OType := OT 9.
+Definition lse_trusted_stack_begin : Addr := A 4096.
+Definition lse_trusted_stack_end : Addr := A 4196.
+Definition lse_stack_begin : Addr := A 1024.
+Definition lse_stack_end : Addr := A 1124.
+
+Ltac unfold_lse_addresses :=
+  unfold lse_main_pcc_begin, lse_main_code_start, lse_main_pcc_end,
+    lse_C_pcc_begin, lse_C_code_start, lse_C_pcc_end,
+    lse_main_data_begin, lse_main_data_end, lse_C_data_begin, lse_C_data_end,
+    lse_main_exports_pcc, lse_main_exports_cgp,
+    lse_main_exports_entries_begin, lse_main_exports_entries_end,
+    lse_C_exports_pcc, lse_C_exports_cgp,
+    lse_C_exports_entries_begin, lse_C_exports_entries_end,
+    lse_assert_begin, lse_assert_cap, lse_assert_end, lse_assert_flag,
+    lse_switcher_begin, lse_switcher_call, lse_switcher_return,
+    lse_switcher_end, lse_switcher_sealing_type,
+    lse_trusted_stack_begin, lse_trusted_stack_end,
+    lse_stack_begin, lse_stack_end.
+
+Ltac unfold_lse_addresses_in H :=
+  unfold lse_main_pcc_begin, lse_main_code_start, lse_main_pcc_end,
+    lse_C_pcc_begin, lse_C_code_start, lse_C_pcc_end,
+    lse_main_data_begin, lse_main_data_end, lse_C_data_begin, lse_C_data_end,
+    lse_main_exports_pcc, lse_main_exports_cgp,
+    lse_main_exports_entries_begin, lse_main_exports_entries_end,
+    lse_C_exports_pcc, lse_C_exports_cgp,
+    lse_C_exports_entries_begin, lse_C_exports_entries_end,
+    lse_assert_begin, lse_assert_cap, lse_assert_end, lse_assert_flag,
+    lse_switcher_begin, lse_switcher_call, lse_switcher_return,
+    lse_switcher_end, lse_switcher_sealing_type,
+    lse_trusted_stack_begin, lse_trusted_stack_end,
+    lse_stack_begin, lse_stack_end in H.
+
+Definition lse_C_load (dst src : RegName) : instr.
+Proof.
+  constructor 5.
+  - exact dst.
+  - exact src.
+Defined.
+
+(** The concrete adversary saves its outer return capability, fetches the
+    switcher and the exported main function, and calls the function twice. It
+    deliberately fetches both imports again before the second call, then
+    restores its return capability and returns to the caller. *)
+Definition lse_C_code : list Word :=
+  encodeInstrsW [
+    Store csp cra; Lea csp 1%Z;
+
+    Mov ct0 PC; GetB cs0 ct0; GetA cs1 ct0; Sub cs0 cs0 cs1;
+    Lea ct0 cs0; Lea ct0 0%Z; lse_C_load ct0 ct0; Mov cs0 0%Z;
+    Mov ct1 PC; GetB cs0 ct1; GetA cs1 ct1; Sub cs0 cs0 cs1;
+    Lea ct1 cs0; Lea ct1 1%Z; lse_C_load ct1 ct1; Mov cs0 0%Z;
+    Jalr cra ct0;
+
+    Mov ct0 PC; GetB cs0 ct0; GetA cs1 ct0; Sub cs0 cs0 cs1;
+    Lea ct0 cs0; Lea ct0 0%Z; lse_C_load ct0 ct0; Mov cs0 0%Z;
+    Mov ct1 PC; GetB cs0 ct1; GetA cs1 ct1; Sub cs0 cs0 cs1;
+    Lea ct1 cs0; Lea ct1 1%Z; lse_C_load ct1 ct1; Mov cs0 0%Z;
+    Jalr cra ct0;
+
+    Lea csp (-1)%Z; lse_C_load cra csp;
+    Mov ca0 0%Z; Mov ca1 0%Z; Jalr cnull cra
+  ].
+
+Definition lse_C_data : list Word := [WInt 0].
+
+Program Definition lse_concrete_cmptSwitcher : cmptSwitcher.
+Proof.
+  refine (@mkCmptSwitcher machine_parameters_instance
+    lse_switcher_begin lse_switcher_end
+    lse_switcher_call lse_switcher_return lse_switcher_sealing_type
+    lse_trusted_stack_begin lse_trusted_stack_end
+    _ _ _ _
+    (replicate 100 (WInt 0)) _ eq_refl
+    lse_stack_begin lse_stack_end (replicate 100 (WInt 0)) _ _).
+  - vm_compute; solve_addr.
+  - vm_compute; solve_addr.
+  - vm_compute; solve_addr.
+  - vm_compute; solve_addr.
+  - vm_compute; solve_addr.
+  - vm_compute; solve_addr.
+  - unfold_lse_addresses.
+    repeat split; unfold disjoint, set_disjoint_instance;
+      intros x Hx Hx'; rewrite !elem_of_finz_seq_between in Hx, Hx';
+      solve_addr.
+Defined.
+
+Program Definition lse_concrete_cmptAssert : cmptAssert.
+Proof.
+  refine (@mkCmptAssert machine_parameters_instance
+    lse_assert_begin lse_assert_end lse_assert_cap lse_assert_flag _ _ _ _).
+  - vm_compute; solve_addr.
+  - vm_compute; solve_addr.
+  - vm_compute; solve_addr.
+  - unfold_lse_addresses.
+    unfold disjoint, set_disjoint_instance.
+    intros x Hx Hx'.
+    rewrite !elem_of_finz_seq_between in Hx, Hx'.
+    solve_addr.
+Defined.
+
+Local Instance lse_concrete_switcherLayout : switcherLayout.
+Proof.
+  exact (cmptSwitcher_switcherLayout lse_concrete_cmptSwitcher).
+Defined.
+
+Local Instance lse_concrete_assertLayout : assertLayout.
+Proof.
+  exact (cmptAssert_assertLayout lse_concrete_cmptAssert).
+Defined.
+
+Definition lse_C_f : Sealable :=
+  SCap RO Global lse_C_exports_pcc lse_C_exports_entries_end
+    lse_C_exports_entries_begin.
+
+Definition lse_main_imports_concrete : list Word := lse_main_imports lse_C_f.
+
+Definition lse_C_imports : list Word :=
+  [ WSentry XSRW_ Local lse_switcher_begin lse_switcher_end lse_switcher_call
+  ; WSealed lse_switcher_sealing_type
+      (lse_entry_f_sb lse_main_exports_pcc lse_main_exports_entries_end)
+  ].
+
+Definition lse_C_exports : list Word := [WInt (encode_entry_point 0 2)].
+
+Program Definition lse_concrete_main_cmpt : cmpt.
+Proof.
+  refine (@mkCmpt
+    lse_main_pcc_begin lse_main_code_start lse_main_pcc_end
+    lse_main_data_begin lse_main_data_end
+    lse_main_exports_pcc lse_main_exports_cgp
+    lse_main_exports_entries_begin lse_main_exports_entries_end
+    lse_main_imports_concrete lse_main_code lse_main_data lse_export_table_entries
+    _ _ _ _ _ _ _).
+  - vm_compute; solve_addr.
+  - vm_compute; solve_addr.
+  - vm_compute; solve_addr.
+  - vm_compute; solve_addr.
+  - vm_compute; solve_addr.
+  - vm_compute; solve_addr.
+  - unfold_lse_addresses; disj_regions.
+Defined.
+
+Program Definition lse_concrete_C_cmpt : cmpt.
+Proof.
+  refine (@mkCmpt
+    lse_C_pcc_begin lse_C_code_start lse_C_pcc_end
+    lse_C_data_begin lse_C_data_end
+    lse_C_exports_pcc lse_C_exports_cgp
+    lse_C_exports_entries_begin lse_C_exports_entries_end
+    lse_C_imports lse_C_code lse_C_data lse_C_exports
+    _ _ _ _ _ _ _).
+  - vm_compute; solve_addr.
+  - vm_compute; solve_addr.
+  - vm_compute; solve_addr.
+  - vm_compute; solve_addr.
+  - vm_compute; solve_addr.
+  - vm_compute; solve_addr.
+  - unfold_lse_addresses; disj_regions.
+Defined.
+
+Ltac solve_lse_concrete_disjoint :=
+  unfold disjoint_cmpt, switcher_cmpt_disjoint, assert_cmpt_disjoint,
+       assert_switcher_disjoint, cmpt_region, cmpt_pcc_region, cmpt_cgp_region,
+       cmpt_exp_tbl_region, cmpt_switcher_region, cmpt_switcher_code_region,
+       cmpt_switcher_trusted_stack_region, cmpt_switcher_stack_region,
+       cmpt_assert_region, cmpt_assert_code_region, cmpt_assert_cap_region,
+       cmpt_assert_flag_region, lse_concrete_cmptSwitcher,
+       lse_concrete_cmptAssert, lse_concrete_main_cmpt, lse_concrete_C_cmpt;
+  cbn [cmpt_b_pcc cmpt_e_pcc cmpt_b_cgp cmpt_e_cgp
+       cmpt_exp_tbl_pcc cmpt_exp_tbl_entries_end
+       b_switcher e_switcher b_trusted_stack e_trusted_stack
+       b_stack e_stack b_assert cap_assert e_assert flag_assert];
+  intros x Hx Hx';
+  repeat (rewrite elem_of_app in Hx || rewrite elem_of_app in Hx');
+  repeat (rewrite elem_of_finz_seq_between in Hx ||
+          rewrite elem_of_finz_seq_between in Hx');
+  unfold_lse_addresses_in Hx;
+  unfold_lse_addresses_in Hx';
+  naive_solver (solve_addr).
+
+Global Instance lse_concrete_layout : memory_layout.
+Proof.
+  refine (@Build_memory_layout machine_parameters_instance
+    lse_concrete_cmptSwitcher lse_concrete_cmptAssert
+    lse_concrete_main_cmpt lse_concrete_C_cmpt 2 _ _ _ _).
+  - solve_lse_concrete_disjoint.
+  - split; solve_lse_concrete_disjoint.
+  - split; solve_lse_concrete_disjoint.
+  - solve_lse_concrete_disjoint.
+Defined.
+
+Definition lse_initial_registers : Reg :=
+  <[PC := WCap RX Global lse_main_pcc_begin lse_main_pcc_end lse_main_code_start]>
+  (<[cgp := WCap RW Global lse_main_data_begin lse_main_data_end
+      lse_main_data_begin]>
+  (<[csp := WCap RWL Local lse_stack_begin lse_stack_end lse_stack_begin]>
+    (gset_to_gmap (WInt 0) all_registers_s))).
+
+Definition lse_initial_sregisters : SReg :=
+  <[MTDC := WCap RWL Local lse_trusted_stack_begin lse_trusted_stack_end
+      lse_trusted_stack_begin]> ∅.
+
+Definition lse_initial_memory : Mem := mk_initial_memory.
+
+Lemma lse_initial_registers_correct :
+  is_initial_registers lse_initial_registers.
+Proof.
+  rewrite /is_initial_registers /lse_initial_registers.
+  cbn [lse_concrete_layout lse_concrete_main_cmpt].
+  split; [|split; [|split]].
+  - vm_compute; reflexivity.
+  - vm_compute; reflexivity.
+  - vm_compute; reflexivity.
+  - intros r Hr; rewrite !lookup_insert_ne; try set_solver.
+    apply lookup_gset_to_gmap_Some; split.
+    + apply all_registers_s_correct.
+    + done.
+Qed.
+
+Lemma lse_initial_sregisters_correct :
+  is_initial_sregisters lse_initial_sregisters.
+Proof.
+  rewrite /is_initial_sregisters /lse_initial_sregisters.
+  cbn [lse_concrete_layout lse_concrete_cmptSwitcher].
+  simplify_map_eq; vm_compute; reflexivity.
+Qed.
+
+Lemma lse_initial_memory_correct : is_initial_memory lse_initial_memory.
+Proof.
+  rewrite /is_initial_memory /lse_initial_memory.
+  repeat split; try reflexivity.
+  - rewrite /lse_C_code /encodeInstrsW; repeat constructor; done.
+  - rewrite /lse_C_data; repeat constructor; done.
+  - apply Forall_replicate; done.
+Qed.
+
+Theorem lse_concrete_adequacy reg' sreg' mem' es :
+  rtc erased_step
+    ([Seq (Instr Executable)],
+      (lse_initial_registers, lse_initial_sregisters, lse_initial_memory))
+    (es, (reg', sreg', mem')) ->
+  mem' !! lse_assert_flag = Some (WInt 0%Z).
+Proof.
+  intro Hrun.
+  pose proof
+    (@lse_adequacy machine_parameters_instance lse_concrete_layout
+      lse_initial_registers reg' lse_initial_sregisters sreg'
+      lse_initial_memory mem' es
+      lse_initial_registers_correct lse_initial_sregisters_correct
+      lse_initial_memory_correct Hrun) as Hadequacy.
+  cbn [lse_concrete_layout lse_concrete_cmptAssert] in Hadequacy.
+  exact Hadequacy.
+Qed.
+
+(** Combining the computed execution with [lse_concrete_adequacy] shows that
+    there is a final machine state such that the exact initial configuration:
+    - executes to [Halted], rather than failing or exhausting the chosen fuel;
+    - finishes with the assertion flag still set to zero.
+    Thus this particular adversarial execution terminates normally without
+    violating the case study's assertion. *)
+Theorem lse_runs_and_gracefully_halts :
+  ∃ reg' sreg' mem',
+    rtc erased_step
+      ([Seq (Instr Executable)],
+        (lse_initial_registers, lse_initial_sregisters, lse_initial_memory))
+      ([Instr Halted], (reg', sreg', mem'))
+    ∧ mem' !! lse_assert_flag = Some (WInt 0%Z).
+Proof.
+  pose proof
+    (machine_run_correct 7500 Executable
+      (lse_initial_registers, lse_initial_sregisters, lse_initial_memory)
+      Halted) as Hrun.
+  specialize (Hrun ltac:(vm_compute; reflexivity)).
+  destruct Hrun as [[[reg' sreg'] mem'] Hrun].
+  exists reg', sreg', mem'. split.
+  - exact Hrun.
+  - eapply lse_concrete_adequacy; exact Hrun.
+Qed.
